Advance to the next bug.. 10 lines further

src/ocaml-output/FStar_Syntax_Util.ml
@@ -442,6 +442,11 @@ let is_tot_or_gtot_comp c =
     (FStar_Ident.lid_equals FStar_Syntax_Const.effect_GTot_lid
        (comp_effect_name c))
   
+let is_named_tot_or_gtot_comp c =
+  let m = comp_effect_name c  in
+  (FStar_Ident.lid_equals FStar_Syntax_Const.effect_Tot_lid m) ||
+    (FStar_Ident.lid_equals FStar_Syntax_Const.effect_GTot_lid m)
+  
 let is_pure_effect : FStar_Ident.lident -> Prims.bool =
   fun l  ->
     ((FStar_Ident.lid_equals l FStar_Syntax_Const.effect_Tot_lid) ||
@@ -450,18 +455,18 @@ let is_pure_effect : FStar_Ident.lident -> Prims.bool =
   
 let is_pure_comp c =
   match c.FStar_Syntax_Syntax.n with
-  | FStar_Syntax_Syntax.Total uu____767 -> true
-  | FStar_Syntax_Syntax.GTotal uu____773 -> false
+  | FStar_Syntax_Syntax.Total uu____779 -> true
+  | FStar_Syntax_Syntax.GTotal uu____785 -> false
   | FStar_Syntax_Syntax.Comp ct ->
       ((is_total_comp c) ||
          (is_pure_effect ct.FStar_Syntax_Syntax.comp_typ_name))
         ||
         (FStar_All.pipe_right ct.FStar_Syntax_Syntax.flags
            (FStar_Util.for_some
-              (fun uu___170_781  ->
-                 match uu___170_781 with
+              (fun uu___170_793  ->
+                 match uu___170_793 with
                  | FStar_Syntax_Syntax.LEMMA  -> true
-                 | uu____782 -> false)))
+                 | uu____794 -> false)))
   
 let is_ghost_effect : FStar_Ident.lident -> Prims.bool =
   fun l  ->
@@ -478,10 +483,10 @@ let is_pure_lcomp : FStar_Syntax_Syntax.lcomp -> Prims.bool =
       ||
       (FStar_All.pipe_right lc.FStar_Syntax_Syntax.lcomp_cflags
          (FStar_Util.for_some
-            (fun uu___171_801  ->
-               match uu___171_801 with
+            (fun uu___171_813  ->
+               match uu___171_813 with
                | FStar_Syntax_Syntax.LEMMA  -> true
-               | uu____802 -> false)))
+               | uu____814 -> false)))
   
 let is_pure_or_ghost_lcomp : FStar_Syntax_Syntax.lcomp -> Prims.bool =
   fun lc  ->
@@ -489,26 +494,26 @@ let is_pure_or_ghost_lcomp : FStar_Syntax_Syntax.lcomp -> Prims.bool =
   
 let is_pure_or_ghost_function : FStar_Syntax_Syntax.term -> Prims.bool =
   fun t  ->
-    let uu____809 =
-      let uu____810 = FStar_Syntax_Subst.compress t  in
-      uu____810.FStar_Syntax_Syntax.n  in
-    match uu____809 with
-    | FStar_Syntax_Syntax.Tm_arrow (uu____813,c) -> is_pure_or_ghost_comp c
-    | uu____825 -> true
+    let uu____821 =
+      let uu____822 = FStar_Syntax_Subst.compress t  in
+      uu____822.FStar_Syntax_Syntax.n  in
+    match uu____821 with
+    | FStar_Syntax_Syntax.Tm_arrow (uu____825,c) -> is_pure_or_ghost_comp c
+    | uu____837 -> true
   
 let is_lemma : FStar_Syntax_Syntax.term -> Prims.bool =
   fun t  ->
-    let uu____829 =
-      let uu____830 = FStar_Syntax_Subst.compress t  in
-      uu____830.FStar_Syntax_Syntax.n  in
-    match uu____829 with
-    | FStar_Syntax_Syntax.Tm_arrow (uu____833,c) ->
+    let uu____841 =
+      let uu____842 = FStar_Syntax_Subst.compress t  in
+      uu____842.FStar_Syntax_Syntax.n  in
+    match uu____841 with
+    | FStar_Syntax_Syntax.Tm_arrow (uu____845,c) ->
         (match c.FStar_Syntax_Syntax.n with
          | FStar_Syntax_Syntax.Comp ct ->
              FStar_Ident.lid_equals ct.FStar_Syntax_Syntax.comp_typ_name
                FStar_Syntax_Const.effect_Lemma_lid
-         | uu____846 -> false)
-    | uu____847 -> false
+         | uu____858 -> false)
+    | uu____859 -> false
   
 let head_and_args :
   FStar_Syntax_Syntax.term ->
@@ -521,45 +526,45 @@ let head_and_args :
     let t1 = FStar_Syntax_Subst.compress t  in
     match t1.FStar_Syntax_Syntax.n with
     | FStar_Syntax_Syntax.Tm_app (head1,args) -> (head1, args)
-    | uu____893 -> (t1, [])
+    | uu____905 -> (t1, [])
   
 let un_uinst : FStar_Syntax_Syntax.term -> FStar_Syntax_Syntax.term =
   fun t  ->
     let t1 = FStar_Syntax_Subst.compress t  in
     match t1.FStar_Syntax_Syntax.n with
-    | FStar_Syntax_Syntax.Tm_uinst (t2,uu____908) ->
+    | FStar_Syntax_Syntax.Tm_uinst (t2,uu____920) ->
         FStar_Syntax_Subst.compress t2
-    | uu____913 -> t1
+    | uu____925 -> t1
   
 let is_smt_lemma : FStar_Syntax_Syntax.term -> Prims.bool =
   fun t  ->
-    let uu____917 =
-      let uu____918 = FStar_Syntax_Subst.compress t  in
-      uu____918.FStar_Syntax_Syntax.n  in
-    match uu____917 with
-    | FStar_Syntax_Syntax.Tm_arrow (uu____921,c) ->
+    let uu____929 =
+      let uu____930 = FStar_Syntax_Subst.compress t  in
+      uu____930.FStar_Syntax_Syntax.n  in
+    match uu____929 with
+    | FStar_Syntax_Syntax.Tm_arrow (uu____933,c) ->
         (match c.FStar_Syntax_Syntax.n with
          | FStar_Syntax_Syntax.Comp ct when
              FStar_Ident.lid_equals ct.FStar_Syntax_Syntax.comp_typ_name
                FStar_Syntax_Const.effect_Lemma_lid
              ->
              (match ct.FStar_Syntax_Syntax.effect_args with
-              | _req::_ens::(pats,uu____937)::uu____938 ->
+              | _req::_ens::(pats,uu____949)::uu____950 ->
                   let pats' = unmeta pats  in
-                  let uu____969 = head_and_args pats'  in
-                  (match uu____969 with
-                   | (head1,uu____980) ->
-                       let uu____995 =
-                         let uu____996 = un_uinst head1  in
-                         uu____996.FStar_Syntax_Syntax.n  in
-                       (match uu____995 with
+                  let uu____981 = head_and_args pats'  in
+                  (match uu____981 with
+                   | (head1,uu____992) ->
+                       let uu____1007 =
+                         let uu____1008 = un_uinst head1  in
+                         uu____1008.FStar_Syntax_Syntax.n  in
+                       (match uu____1007 with
                         | FStar_Syntax_Syntax.Tm_fvar fv ->
                             FStar_Syntax_Syntax.fv_eq_lid fv
                               FStar_Syntax_Const.cons_lid
-                        | uu____1000 -> false))
-              | uu____1001 -> false)
-         | uu____1007 -> false)
-    | uu____1008 -> false
+                        | uu____1012 -> false))
+              | uu____1013 -> false)
+         | uu____1019 -> false)
+    | uu____1020 -> false
   
 let is_ml_comp c =
   match c.FStar_Syntax_Syntax.n with
@@ -569,18 +574,18 @@ let is_ml_comp c =
         ||
         (FStar_All.pipe_right c1.FStar_Syntax_Syntax.flags
            (FStar_Util.for_some
-              (fun uu___172_1022  ->
-                 match uu___172_1022 with
+              (fun uu___172_1034  ->
+                 match uu___172_1034 with
                  | FStar_Syntax_Syntax.MLEFFECT  -> true
-                 | uu____1023 -> false)))
-  | uu____1024 -> false 
+                 | uu____1035 -> false)))
+  | uu____1036 -> false 
 let is_trivial_wp c =
   FStar_All.pipe_right (comp_flags c)
     (FStar_Util.for_some
-       (fun uu___173_1037  ->
-          match uu___173_1037 with
+       (fun uu___173_1049  ->
+          match uu___173_1049 with
           | FStar_Syntax_Syntax.TOTAL |FStar_Syntax_Syntax.RETURN  -> true
-          | uu____1038 -> false))
+          | uu____1050 -> false))
   
 let primops : FStar_Ident.lident Prims.list =
   [FStar_Syntax_Const.op_Eq;
@@ -607,20 +612,20 @@ let is_primop f =
   match f.FStar_Syntax_Syntax.n with
   | FStar_Syntax_Syntax.Tm_fvar fv ->
       is_primop_lid (fv.FStar_Syntax_Syntax.fv_name).FStar_Syntax_Syntax.v
-  | uu____1060 -> false 
+  | uu____1072 -> false 
 let rec unascribe : FStar_Syntax_Syntax.term -> FStar_Syntax_Syntax.term =
   fun e  ->
     let e1 = FStar_Syntax_Subst.compress e  in
     match e1.FStar_Syntax_Syntax.n with
-    | FStar_Syntax_Syntax.Tm_ascribed (e2,uu____1066,uu____1067) ->
+    | FStar_Syntax_Syntax.Tm_ascribed (e2,uu____1078,uu____1079) ->
         unascribe e2
-    | uu____1086 -> e1
+    | uu____1098 -> e1
   
 let rec ascribe t k =
   match t.FStar_Syntax_Syntax.n with
-  | FStar_Syntax_Syntax.Tm_ascribed (t',uu____1118,uu____1119) ->
+  | FStar_Syntax_Syntax.Tm_ascribed (t',uu____1130,uu____1131) ->
       ascribe t' k
-  | uu____1138 ->
+  | uu____1150 ->
       FStar_Syntax_Syntax.mk (FStar_Syntax_Syntax.Tm_ascribed (t, k, None))
         None t.FStar_Syntax_Syntax.pos
   
@@ -630,15 +635,15 @@ type eq_result =
   | Unknown 
 let uu___is_Equal : eq_result -> Prims.bool =
   fun projectee  ->
-    match projectee with | Equal  -> true | uu____1155 -> false
+    match projectee with | Equal  -> true | uu____1167 -> false
   
 let uu___is_NotEqual : eq_result -> Prims.bool =
   fun projectee  ->
-    match projectee with | NotEqual  -> true | uu____1159 -> false
+    match projectee with | NotEqual  -> true | uu____1171 -> false
   
 let uu___is_Unknown : eq_result -> Prims.bool =
   fun projectee  ->
-    match projectee with | Unknown  -> true | uu____1163 -> false
+    match projectee with | Unknown  -> true | uu____1175 -> false
   
 let rec eq_tm :
   FStar_Syntax_Syntax.term -> FStar_Syntax_Syntax.term -> eq_result =
@@ -646,42 +651,42 @@ let rec eq_tm :
     fun t2  ->
       let t11 = unascribe t1  in
       let t21 = unascribe t2  in
-      let equal_if uu___174_1183 = if uu___174_1183 then Equal else Unknown
+      let equal_if uu___174_1195 = if uu___174_1195 then Equal else Unknown
          in
-      let equal_iff uu___175_1188 = if uu___175_1188 then Equal else NotEqual
+      let equal_iff uu___175_1200 = if uu___175_1200 then Equal else NotEqual
          in
-      let eq_and f g = match f with | Equal  -> g () | uu____1202 -> Unknown
+      let eq_and f g = match f with | Equal  -> g () | uu____1214 -> Unknown
          in
       match ((t11.FStar_Syntax_Syntax.n), (t21.FStar_Syntax_Syntax.n)) with
       | (FStar_Syntax_Syntax.Tm_name a,FStar_Syntax_Syntax.Tm_name b) ->
           equal_if (FStar_Syntax_Syntax.bv_eq a b)
       | (FStar_Syntax_Syntax.Tm_fvar f,FStar_Syntax_Syntax.Tm_fvar g) ->
-          let uu____1207 = FStar_Syntax_Syntax.fv_eq f g  in
-          equal_if uu____1207
+          let uu____1219 = FStar_Syntax_Syntax.fv_eq f g  in
+          equal_if uu____1219
       | (FStar_Syntax_Syntax.Tm_uinst (f,us),FStar_Syntax_Syntax.Tm_uinst
          (g,vs)) ->
-          let uu____1220 = eq_tm f g  in
-          eq_and uu____1220
-            (fun uu____1221  ->
-               let uu____1222 = eq_univs_list us vs  in equal_if uu____1222)
+          let uu____1232 = eq_tm f g  in
+          eq_and uu____1232
+            (fun uu____1233  ->
+               let uu____1234 = eq_univs_list us vs  in equal_if uu____1234)
       | (FStar_Syntax_Syntax.Tm_constant c,FStar_Syntax_Syntax.Tm_constant d)
           ->
-          let uu____1225 = FStar_Const.eq_const c d  in equal_iff uu____1225
+          let uu____1237 = FStar_Const.eq_const c d  in equal_iff uu____1237
       | (FStar_Syntax_Syntax.Tm_uvar
-         (u1,uu____1227),FStar_Syntax_Syntax.Tm_uvar (u2,uu____1229)) ->
-          let uu____1254 = FStar_Unionfind.equivalent u1 u2  in
-          equal_if uu____1254
+         (u1,uu____1239),FStar_Syntax_Syntax.Tm_uvar (u2,uu____1241)) ->
+          let uu____1266 = FStar_Unionfind.equivalent u1 u2  in
+          equal_if uu____1266
       | (FStar_Syntax_Syntax.Tm_app (h1,args1),FStar_Syntax_Syntax.Tm_app
          (h2,args2)) ->
-          let uu____1290 = eq_tm h1 h2  in
-          eq_and uu____1290 (fun uu____1291  -> eq_args args1 args2)
+          let uu____1302 = eq_tm h1 h2  in
+          eq_and uu____1302 (fun uu____1303  -> eq_args args1 args2)
       | (FStar_Syntax_Syntax.Tm_type u,FStar_Syntax_Syntax.Tm_type v1) ->
-          let uu____1294 = eq_univs u v1  in equal_if uu____1294
-      | (FStar_Syntax_Syntax.Tm_meta (t12,uu____1296),uu____1297) ->
+          let uu____1306 = eq_univs u v1  in equal_if uu____1306
+      | (FStar_Syntax_Syntax.Tm_meta (t12,uu____1308),uu____1309) ->
           eq_tm t12 t21
-      | (uu____1302,FStar_Syntax_Syntax.Tm_meta (t22,uu____1304)) ->
+      | (uu____1314,FStar_Syntax_Syntax.Tm_meta (t22,uu____1316)) ->
           eq_tm t11 t22
-      | uu____1309 -> Unknown
+      | uu____1321 -> Unknown
 
 and eq_args :
   FStar_Syntax_Syntax.args -> FStar_Syntax_Syntax.args -> eq_result =
@@ -689,12 +694,12 @@ and eq_args :
     fun a2  ->
       match (a1, a2) with
       | ([],[]) -> Equal
-      | ((a,uu____1333)::a11,(b,uu____1336)::b1) ->
-          let uu____1374 = eq_tm a b  in
-          (match uu____1374 with
+      | ((a,uu____1345)::a11,(b,uu____1348)::b1) ->
+          let uu____1386 = eq_tm a b  in
+          (match uu____1386 with
            | Equal  -> eq_args a11 b1
-           | uu____1375 -> Unknown)
-      | uu____1376 -> Unknown
+           | uu____1387 -> Unknown)
+      | uu____1388 -> Unknown
 
 and eq_univs_list :
   FStar_Syntax_Syntax.universes ->
@@ -709,51 +714,51 @@ let rec unrefine : FStar_Syntax_Syntax.term -> FStar_Syntax_Syntax.term =
   fun t  ->
     let t1 = FStar_Syntax_Subst.compress t  in
     match t1.FStar_Syntax_Syntax.n with
-    | FStar_Syntax_Syntax.Tm_refine (x,uu____1390) ->
+    | FStar_Syntax_Syntax.Tm_refine (x,uu____1402) ->
         unrefine x.FStar_Syntax_Syntax.sort
-    | FStar_Syntax_Syntax.Tm_ascribed (t2,uu____1396,uu____1397) ->
+    | FStar_Syntax_Syntax.Tm_ascribed (t2,uu____1408,uu____1409) ->
         unrefine t2
-    | uu____1416 -> t1
+    | uu____1428 -> t1
   
 let rec is_unit : FStar_Syntax_Syntax.term -> Prims.bool =
   fun t  ->
-    let uu____1420 =
-      let uu____1421 = unrefine t  in uu____1421.FStar_Syntax_Syntax.n  in
-    match uu____1420 with
-    | FStar_Syntax_Syntax.Tm_type uu____1424 -> true
+    let uu____1432 =
+      let uu____1433 = unrefine t  in uu____1433.FStar_Syntax_Syntax.n  in
+    match uu____1432 with
+    | FStar_Syntax_Syntax.Tm_type uu____1436 -> true
     | FStar_Syntax_Syntax.Tm_fvar fv ->
         (FStar_Syntax_Syntax.fv_eq_lid fv FStar_Syntax_Const.unit_lid) ||
           (FStar_Syntax_Syntax.fv_eq_lid fv FStar_Syntax_Const.squash_lid)
-    | FStar_Syntax_Syntax.Tm_uinst (t1,uu____1427) -> is_unit t1
-    | uu____1432 -> false
+    | FStar_Syntax_Syntax.Tm_uinst (t1,uu____1439) -> is_unit t1
+    | uu____1444 -> false
   
 let is_fun : FStar_Syntax_Syntax.term -> Prims.bool =
   fun e  ->
-    let uu____1436 =
-      let uu____1437 = FStar_Syntax_Subst.compress e  in
-      uu____1437.FStar_Syntax_Syntax.n  in
-    match uu____1436 with
-    | FStar_Syntax_Syntax.Tm_abs uu____1440 -> true
-    | uu____1455 -> false
+    let uu____1448 =
+      let uu____1449 = FStar_Syntax_Subst.compress e  in
+      uu____1449.FStar_Syntax_Syntax.n  in
+    match uu____1448 with
+    | FStar_Syntax_Syntax.Tm_abs uu____1452 -> true
+    | uu____1467 -> false
   
 let is_function_typ : FStar_Syntax_Syntax.term -> Prims.bool =
   fun t  ->
-    let uu____1459 =
-      let uu____1460 = FStar_Syntax_Subst.compress t  in
-      uu____1460.FStar_Syntax_Syntax.n  in
-    match uu____1459 with
-    | FStar_Syntax_Syntax.Tm_arrow uu____1463 -> true
-    | uu____1471 -> false
+    let uu____1471 =
+      let uu____1472 = FStar_Syntax_Subst.compress t  in
+      uu____1472.FStar_Syntax_Syntax.n  in
+    match uu____1471 with
+    | FStar_Syntax_Syntax.Tm_arrow uu____1475 -> true
+    | uu____1483 -> false
   
 let rec pre_typ : FStar_Syntax_Syntax.term -> FStar_Syntax_Syntax.term =
   fun t  ->
     let t1 = FStar_Syntax_Subst.compress t  in
     match t1.FStar_Syntax_Syntax.n with
-    | FStar_Syntax_Syntax.Tm_refine (x,uu____1477) ->
+    | FStar_Syntax_Syntax.Tm_refine (x,uu____1489) ->
         pre_typ x.FStar_Syntax_Syntax.sort
-    | FStar_Syntax_Syntax.Tm_ascribed (t2,uu____1483,uu____1484) ->
+    | FStar_Syntax_Syntax.Tm_ascribed (t2,uu____1495,uu____1496) ->
         pre_typ t2
-    | uu____1503 -> t1
+    | uu____1515 -> t1
   
 let destruct :
   FStar_Syntax_Syntax.term ->
@@ -765,19 +770,19 @@ let destruct :
   fun typ  ->
     fun lid  ->
       let typ1 = FStar_Syntax_Subst.compress typ  in
-      let uu____1517 =
-        let uu____1518 = un_uinst typ1  in uu____1518.FStar_Syntax_Syntax.n
+      let uu____1529 =
+        let uu____1530 = un_uinst typ1  in uu____1530.FStar_Syntax_Syntax.n
          in
-      match uu____1517 with
+      match uu____1529 with
       | FStar_Syntax_Syntax.Tm_app (head1,args) ->
           let head2 = un_uinst head1  in
           (match head2.FStar_Syntax_Syntax.n with
            | FStar_Syntax_Syntax.Tm_fvar tc when
                FStar_Syntax_Syntax.fv_eq_lid tc lid -> Some args
-           | uu____1556 -> None)
+           | uu____1568 -> None)
       | FStar_Syntax_Syntax.Tm_fvar tc when
           FStar_Syntax_Syntax.fv_eq_lid tc lid -> Some []
-      | uu____1572 -> None
+      | uu____1584 -> None
   
 let lids_of_sigelt :
   FStar_Syntax_Syntax.sigelt -> FStar_Ident.lident Prims.list =
@@ -800,7 +805,7 @@ let lids_of_sigelt :
 let lid_of_sigelt :
   FStar_Syntax_Syntax.sigelt -> FStar_Ident.lident Prims.option =
   fun se  ->
-    match lids_of_sigelt se with | l::[] -> Some l | uu____1649 -> None
+    match lids_of_sigelt se with | l::[] -> Some l | uu____1661 -> None
   
 let quals_of_sigelt :
   FStar_Syntax_Syntax.sigelt -> FStar_Syntax_Syntax.qualifier Prims.list =
@@ -875,13 +880,13 @@ let range_of_sigelt : FStar_Syntax_Syntax.sigelt -> FStar_Range.range =
                 |FStar_Syntax_Syntax.Sig_sub_effect (_,r)
         -> r
   
-let range_of_lb uu___176_1832 =
-  match uu___176_1832 with
-  | (FStar_Util.Inl x,uu____1839,uu____1840) ->
+let range_of_lb uu___176_1844 =
+  match uu___176_1844 with
+  | (FStar_Util.Inl x,uu____1851,uu____1852) ->
       FStar_Syntax_Syntax.range_of_bv x
-  | (FStar_Util.Inr l,uu____1844,uu____1845) -> FStar_Ident.range_of_lid l 
-let range_of_arg uu____1862 =
-  match uu____1862 with | (hd1,uu____1868) -> hd1.FStar_Syntax_Syntax.pos 
+  | (FStar_Util.Inr l,uu____1856,uu____1857) -> FStar_Ident.range_of_lid l 
+let range_of_arg uu____1874 =
+  match uu____1874 with | (hd1,uu____1880) -> hd1.FStar_Syntax_Syntax.pos 
 let range_of_args args r =
   FStar_All.pipe_right args
     (FStar_List.fold_left
@@ -893,27 +898,27 @@ let mk_app f args =
 let mk_data l args =
   match args with
   | [] ->
-      let uu____1982 =
-        let uu____1985 =
-          let uu____1986 =
-            let uu____1991 =
+      let uu____1994 =
+        let uu____1997 =
+          let uu____1998 =
+            let uu____2003 =
               FStar_Syntax_Syntax.fvar l FStar_Syntax_Syntax.Delta_constant
                 (Some FStar_Syntax_Syntax.Data_ctor)
                in
-            (uu____1991,
+            (uu____2003,
               (FStar_Syntax_Syntax.Meta_desugared
                  FStar_Syntax_Syntax.Data_app))
              in
-          FStar_Syntax_Syntax.Tm_meta uu____1986  in
-        FStar_Syntax_Syntax.mk uu____1985  in
-      uu____1982 None (FStar_Ident.range_of_lid l)
-  | uu____2000 ->
+          FStar_Syntax_Syntax.Tm_meta uu____1998  in
+        FStar_Syntax_Syntax.mk uu____1997  in
+      uu____1994 None (FStar_Ident.range_of_lid l)
+  | uu____2012 ->
       let e =
-        let uu____2009 =
+        let uu____2021 =
           FStar_Syntax_Syntax.fvar l FStar_Syntax_Syntax.Delta_constant
             (Some FStar_Syntax_Syntax.Data_ctor)
            in
-        mk_app uu____2009 args  in
+        mk_app uu____2021 args  in
       FStar_Syntax_Syntax.mk
         (FStar_Syntax_Syntax.Tm_meta
            (e,
@@ -930,13 +935,13 @@ let unmangle_field_name : FStar_Ident.ident -> FStar_Ident.ident =
   fun x  ->
     if FStar_Util.starts_with x.FStar_Ident.idText "^fname^"
     then
-      let uu____2024 =
-        let uu____2027 =
+      let uu____2036 =
+        let uu____2039 =
           FStar_Util.substring_from x.FStar_Ident.idText
             (Prims.parse_int "7")
            in
-        (uu____2027, (x.FStar_Ident.idRange))  in
-      FStar_Ident.mk_ident uu____2024
+        (uu____2039, (x.FStar_Ident.idRange))  in
+      FStar_Ident.mk_ident uu____2036
     else x
   
 let field_projector_prefix : Prims.string = "__proj__" 
@@ -976,40 +981,40 @@ let mk_field_projector_name :
     fun x  ->
       fun i  ->
         let nm =
-          let uu____2060 = FStar_Syntax_Syntax.is_null_bv x  in
-          if uu____2060
+          let uu____2072 = FStar_Syntax_Syntax.is_null_bv x  in
+          if uu____2072
           then
-            let uu____2061 =
-              let uu____2064 =
-                let uu____2065 = FStar_Util.string_of_int i  in
-                Prims.strcat "_" uu____2065  in
-              let uu____2066 = FStar_Syntax_Syntax.range_of_bv x  in
-              (uu____2064, uu____2066)  in
-            FStar_Ident.mk_ident uu____2061
+            let uu____2073 =
+              let uu____2076 =
+                let uu____2077 = FStar_Util.string_of_int i  in
+                Prims.strcat "_" uu____2077  in
+              let uu____2078 = FStar_Syntax_Syntax.range_of_bv x  in
+              (uu____2076, uu____2078)  in
+            FStar_Ident.mk_ident uu____2073
           else x.FStar_Syntax_Syntax.ppname  in
         let y =
-          let uu___179_2069 = x  in
+          let uu___179_2081 = x  in
           {
             FStar_Syntax_Syntax.ppname = nm;
             FStar_Syntax_Syntax.index =
-              (uu___179_2069.FStar_Syntax_Syntax.index);
+              (uu___179_2081.FStar_Syntax_Syntax.index);
             FStar_Syntax_Syntax.sort =
-              (uu___179_2069.FStar_Syntax_Syntax.sort)
+              (uu___179_2081.FStar_Syntax_Syntax.sort)
           }  in
-        let uu____2070 = mk_field_projector_name_from_ident lid nm  in
-        (uu____2070, y)
+        let uu____2082 = mk_field_projector_name_from_ident lid nm  in
+        (uu____2082, y)
   
 let set_uvar uv t =
-  let uu____2087 = FStar_Unionfind.find uv  in
-  match uu____2087 with
-  | FStar_Syntax_Syntax.Fixed uu____2090 ->
-      let uu____2091 =
-        let uu____2092 =
-          let uu____2093 = FStar_Unionfind.uvar_id uv  in
-          FStar_All.pipe_left FStar_Util.string_of_int uu____2093  in
-        FStar_Util.format1 "Changing a fixed uvar! ?%s\n" uu____2092  in
-      failwith uu____2091
-  | uu____2095 -> FStar_Unionfind.change uv (FStar_Syntax_Syntax.Fixed t) 
+  let uu____2099 = FStar_Unionfind.find uv  in
+  match uu____2099 with
+  | FStar_Syntax_Syntax.Fixed uu____2102 ->
+      let uu____2103 =
+        let uu____2104 =
+          let uu____2105 = FStar_Unionfind.uvar_id uv  in
+          FStar_All.pipe_left FStar_Util.string_of_int uu____2105  in
+        FStar_Util.format1 "Changing a fixed uvar! ?%s\n" uu____2104  in
+      failwith uu____2103
+  | uu____2107 -> FStar_Unionfind.change uv (FStar_Syntax_Syntax.Fixed t) 
 let qualifier_equal :
   FStar_Syntax_Syntax.qualifier ->
     FStar_Syntax_Syntax.qualifier -> Prims.bool
@@ -1039,7 +1044,7 @@ let qualifier_equal :
                (fun x1  ->
                   fun x2  -> x1.FStar_Ident.idText = x2.FStar_Ident.idText)
                f1 f2)
-      | uu____2142 -> q1 = q2
+      | uu____2154 -> q1 = q2
   
 let abs :
   (FStar_Syntax_Syntax.bv * FStar_Syntax_Syntax.aqual) Prims.list ->
@@ -1058,42 +1063,42 @@ let abs :
              match lopt1 with
              | None |Some (FStar_Util.Inr _) -> lopt1
              | Some (FStar_Util.Inl lc) ->
-                 let uu____2228 =
-                   let uu____2234 = FStar_Syntax_Subst.close_lcomp bs lc  in
-                   FStar_Util.Inl uu____2234  in
-                 Some uu____2228
+                 let uu____2240 =
+                   let uu____2246 = FStar_Syntax_Subst.close_lcomp bs lc  in
+                   FStar_Util.Inl uu____2246  in
+                 Some uu____2240
               in
            match bs with
            | [] -> t
-           | uu____2245 ->
+           | uu____2257 ->
                let body =
-                 let uu____2250 = FStar_Syntax_Subst.close bs t  in
-                 FStar_Syntax_Subst.compress uu____2250  in
+                 let uu____2262 = FStar_Syntax_Subst.close bs t  in
+                 FStar_Syntax_Subst.compress uu____2262  in
                (match ((body.FStar_Syntax_Syntax.n), lopt) with
                 | (FStar_Syntax_Syntax.Tm_abs (bs',t1,lopt'),None ) ->
-                    let uu____2293 =
-                      let uu____2296 =
-                        let uu____2297 =
-                          let uu____2312 =
-                            let uu____2316 =
+                    let uu____2305 =
+                      let uu____2308 =
+                        let uu____2309 =
+                          let uu____2324 =
+                            let uu____2328 =
                               FStar_Syntax_Subst.close_binders bs  in
-                            FStar_List.append uu____2316 bs'  in
-                          let uu____2322 = close_lopt lopt'  in
-                          (uu____2312, t1, uu____2322)  in
-                        FStar_Syntax_Syntax.Tm_abs uu____2297  in
-                      FStar_Syntax_Syntax.mk uu____2296  in
-                    uu____2293 None t1.FStar_Syntax_Syntax.pos
-                | uu____2348 ->
-                    let uu____2357 =
-                      let uu____2360 =
-                        let uu____2361 =
-                          let uu____2376 =
+                            FStar_List.append uu____2328 bs'  in
+                          let uu____2334 = close_lopt lopt'  in
+                          (uu____2324, t1, uu____2334)  in
+                        FStar_Syntax_Syntax.Tm_abs uu____2309  in
+                      FStar_Syntax_Syntax.mk uu____2308  in
+                    uu____2305 None t1.FStar_Syntax_Syntax.pos
+                | uu____2360 ->
+                    let uu____2369 =
+                      let uu____2372 =
+                        let uu____2373 =
+                          let uu____2388 =
                             FStar_Syntax_Subst.close_binders bs  in
-                          let uu____2377 = close_lopt lopt  in
-                          (uu____2376, body, uu____2377)  in
-                        FStar_Syntax_Syntax.Tm_abs uu____2361  in
-                      FStar_Syntax_Syntax.mk uu____2360  in
-                    uu____2357 None t.FStar_Syntax_Syntax.pos))
+                          let uu____2389 = close_lopt lopt  in
+                          (uu____2388, body, uu____2389)  in
+                        FStar_Syntax_Syntax.Tm_abs uu____2373  in
+                      FStar_Syntax_Syntax.mk uu____2372  in
+                    uu____2369 None t.FStar_Syntax_Syntax.pos))
   
 let arrow :
   FStar_Syntax_Syntax.binders ->
@@ -1105,16 +1110,16 @@ let arrow :
     fun c  ->
       match bs with
       | [] -> failwith "Arrow with empty binders"
-      | uu____2406 ->
-          let uu____2407 =
-            let uu____2410 =
-              let uu____2411 =
-                let uu____2419 = FStar_Syntax_Subst.close_binders bs  in
-                let uu____2420 = FStar_Syntax_Subst.close_comp bs c  in
-                (uu____2419, uu____2420)  in
-              FStar_Syntax_Syntax.Tm_arrow uu____2411  in
-            FStar_Syntax_Syntax.mk uu____2410  in
-          uu____2407 None c.FStar_Syntax_Syntax.pos
+      | uu____2418 ->
+          let uu____2419 =
+            let uu____2422 =
+              let uu____2423 =
+                let uu____2431 = FStar_Syntax_Subst.close_binders bs  in
+                let uu____2432 = FStar_Syntax_Subst.close_comp bs c  in
+                (uu____2431, uu____2432)  in
+              FStar_Syntax_Syntax.Tm_arrow uu____2423  in
+            FStar_Syntax_Syntax.mk uu____2422  in
+          uu____2419 None c.FStar_Syntax_Syntax.pos
   
 let maybe_tot_arrow :
   FStar_Syntax_Syntax.binders ->
@@ -1126,17 +1131,17 @@ let maybe_tot_arrow :
     fun t  ->
       match bs with
       | [] -> t
-      | uu____2437 ->
+      | uu____2449 ->
           let c = FStar_Syntax_Syntax.mk_Total t  in
-          let uu____2439 =
-            let uu____2442 =
-              let uu____2443 =
-                let uu____2451 = FStar_Syntax_Subst.close_binders bs  in
-                let uu____2452 = FStar_Syntax_Subst.close_comp bs c  in
-                (uu____2451, uu____2452)  in
-              FStar_Syntax_Syntax.Tm_arrow uu____2443  in
-            FStar_Syntax_Syntax.mk uu____2442  in
-          uu____2439 None c.FStar_Syntax_Syntax.pos
+          let uu____2451 =
+            let uu____2454 =
+              let uu____2455 =
+                let uu____2463 = FStar_Syntax_Subst.close_binders bs  in
+                let uu____2464 = FStar_Syntax_Subst.close_comp bs c  in
+                (uu____2463, uu____2464)  in
+              FStar_Syntax_Syntax.Tm_arrow uu____2455  in
+            FStar_Syntax_Syntax.mk uu____2454  in
+          uu____2451 None c.FStar_Syntax_Syntax.pos
   
 let flat_arrow :
   FStar_Syntax_Syntax.binders ->
@@ -1147,27 +1152,27 @@ let flat_arrow :
   fun bs  ->
     fun c  ->
       let t = arrow bs c  in
-      let uu____2470 =
-        let uu____2471 = FStar_Syntax_Subst.compress t  in
-        uu____2471.FStar_Syntax_Syntax.n  in
-      match uu____2470 with
+      let uu____2482 =
+        let uu____2483 = FStar_Syntax_Subst.compress t  in
+        uu____2483.FStar_Syntax_Syntax.n  in
+      match uu____2482 with
       | FStar_Syntax_Syntax.Tm_arrow (bs1,c1) ->
           (match c1.FStar_Syntax_Syntax.n with
-           | FStar_Syntax_Syntax.Total (tres,uu____2491) ->
-               let uu____2498 =
-                 let uu____2499 = FStar_Syntax_Subst.compress tres  in
-                 uu____2499.FStar_Syntax_Syntax.n  in
-               (match uu____2498 with
+           | FStar_Syntax_Syntax.Total (tres,uu____2503) ->
+               let uu____2510 =
+                 let uu____2511 = FStar_Syntax_Subst.compress tres  in
+                 uu____2511.FStar_Syntax_Syntax.n  in
+               (match uu____2510 with
                 | FStar_Syntax_Syntax.Tm_arrow (bs',c') ->
-                    let uu____2516 = FStar_ST.read t.FStar_Syntax_Syntax.tk
+                    let uu____2528 = FStar_ST.read t.FStar_Syntax_Syntax.tk
                        in
                     (FStar_Syntax_Syntax.mk
                        (FStar_Syntax_Syntax.Tm_arrow
-                          ((FStar_List.append bs1 bs'), c'))) uu____2516
+                          ((FStar_List.append bs1 bs'), c'))) uu____2528
                       t.FStar_Syntax_Syntax.pos
-                | uu____2536 -> t)
-           | uu____2537 -> t)
-      | uu____2538 -> t
+                | uu____2548 -> t)
+           | uu____2549 -> t)
+      | uu____2550 -> t
   
 let refine :
   FStar_Syntax_Syntax.bv ->
@@ -1177,30 +1182,41 @@ let refine :
   =
   fun b  ->
     fun t  ->
-      let uu____2547 =
+      let uu____2559 =
         FStar_ST.read (b.FStar_Syntax_Syntax.sort).FStar_Syntax_Syntax.tk  in
-      let uu____2552 =
-        let uu____2553 = FStar_Syntax_Syntax.range_of_bv b  in
-        FStar_Range.union_ranges uu____2553 t.FStar_Syntax_Syntax.pos  in
-      let uu____2554 =
-        let uu____2557 =
-          let uu____2558 =
-            let uu____2563 =
-              let uu____2564 =
-                let uu____2565 = FStar_Syntax_Syntax.mk_binder b  in
-                [uu____2565]  in
-              FStar_Syntax_Subst.close uu____2564 t  in
-            (b, uu____2563)  in
-          FStar_Syntax_Syntax.Tm_refine uu____2558  in
-        FStar_Syntax_Syntax.mk uu____2557  in
-      uu____2554 uu____2547 uu____2552
+      let uu____2564 =
+        let uu____2565 = FStar_Syntax_Syntax.range_of_bv b  in
+        FStar_Range.union_ranges uu____2565 t.FStar_Syntax_Syntax.pos  in
+      let uu____2566 =
+        let uu____2569 =
+          let uu____2570 =
+            let uu____2575 =
+              let uu____2576 =
+                let uu____2577 = FStar_Syntax_Syntax.mk_binder b  in
+                [uu____2577]  in
+              FStar_Syntax_Subst.close uu____2576 t  in
+            (b, uu____2575)  in
+          FStar_Syntax_Syntax.Tm_refine uu____2570  in
+        FStar_Syntax_Syntax.mk uu____2569  in
+      uu____2566 uu____2559 uu____2564
   
 let branch : FStar_Syntax_Syntax.branch -> FStar_Syntax_Syntax.branch =
   fun b  -> FStar_Syntax_Subst.close_branch b 
 let tot_or_gtot_result c =
   match c.FStar_Syntax_Syntax.n with
   | FStar_Syntax_Syntax.Total (t,_)|FStar_Syntax_Syntax.GTotal (t,_) -> t
-  | uu____2603 -> failwith "Expected a Tot or GTot computation" 
+  | FStar_Syntax_Syntax.Comp c1 ->
+      if
+        (FStar_Ident.lid_equals c1.FStar_Syntax_Syntax.comp_typ_name
+           FStar_Syntax_Const.effect_Tot_lid)
+          ||
+          (FStar_Ident.lid_equals c1.FStar_Syntax_Syntax.comp_typ_name
+             FStar_Syntax_Const.effect_GTot_lid)
+      then
+        let uu____2618 = FStar_List.hd c1.FStar_Syntax_Syntax.effect_args  in
+        FStar_All.pipe_left Prims.fst uu____2618
+      else failwith "Expected a Tot or GTot computation"
+  
 let rec arrow_formals_comp :
   FStar_Syntax_Syntax.term ->
     ((FStar_Syntax_Syntax.bv * FStar_Syntax_Syntax.aqual) Prims.list *
@@ -1210,20 +1226,19 @@ let rec arrow_formals_comp :
     let k1 = FStar_Syntax_Subst.compress k  in
     match k1.FStar_Syntax_Syntax.n with
     | FStar_Syntax_Syntax.Tm_arrow (bs,c) ->
-        let uu____2632 = FStar_Syntax_Subst.open_comp bs c  in
-        (match uu____2632 with
+        let uu____2664 = FStar_Syntax_Subst.open_comp bs c  in
+        (match uu____2664 with
          | (bs1,c1) ->
-             let uu____2642 = is_tot_or_gtot_comp c1  in
-             if uu____2642
+             if is_named_tot_or_gtot_comp c1
              then
-               let uu____2648 =
-                 let uu____2654 = tot_or_gtot_result c1  in
-                 arrow_formals_comp uu____2654  in
-               (match uu____2648 with
+               let uu____2679 =
+                 let uu____2685 = tot_or_gtot_result c1  in
+                 arrow_formals_comp uu____2685  in
+               (match uu____2679 with
                 | (bs',k2) -> ((FStar_List.append bs1 bs'), k2))
              else (bs1, c1))
-    | uu____2674 ->
-        let uu____2675 = FStar_Syntax_Syntax.mk_Total k1  in ([], uu____2675)
+    | uu____2705 ->
+        let uu____2706 = FStar_Syntax_Syntax.mk_Total k1  in ([], uu____2706)
   
 let abs_formals :
   FStar_Syntax_Syntax.term ->
@@ -1237,53 +1252,53 @@ let abs_formals :
       match l with
       | Some (FStar_Util.Inl l1) ->
           let l2 =
-            let uu___180_2736 = l1  in
-            let uu____2737 =
+            let uu___180_2767 = l1  in
+            let uu____2768 =
               FStar_List.map
-                (fun uu____2747  ->
-                   match uu____2747 with
+                (fun uu____2778  ->
+                   match uu____2778 with
                    | (t1,imp) ->
-                       let uu____2754 = FStar_Syntax_Subst.subst s t1  in
-                       (uu____2754, imp))
+                       let uu____2785 = FStar_Syntax_Subst.subst s t1  in
+                       (uu____2785, imp))
                 l1.FStar_Syntax_Syntax.lcomp_indices
                in
-            let uu____2755 =
+            let uu____2786 =
               FStar_Syntax_Subst.subst s l1.FStar_Syntax_Syntax.lcomp_res_typ
                in
             {
               FStar_Syntax_Syntax.lcomp_name =
-                (uu___180_2736.FStar_Syntax_Syntax.lcomp_name);
+                (uu___180_2767.FStar_Syntax_Syntax.lcomp_name);
               FStar_Syntax_Syntax.lcomp_univs =
-                (uu___180_2736.FStar_Syntax_Syntax.lcomp_univs);
-              FStar_Syntax_Syntax.lcomp_indices = uu____2737;
-              FStar_Syntax_Syntax.lcomp_res_typ = uu____2755;
+                (uu___180_2767.FStar_Syntax_Syntax.lcomp_univs);
+              FStar_Syntax_Syntax.lcomp_indices = uu____2768;
+              FStar_Syntax_Syntax.lcomp_res_typ = uu____2786;
               FStar_Syntax_Syntax.lcomp_cflags =
-                (uu___180_2736.FStar_Syntax_Syntax.lcomp_cflags);
+                (uu___180_2767.FStar_Syntax_Syntax.lcomp_cflags);
               FStar_Syntax_Syntax.lcomp_as_comp =
-                (fun uu____2758  ->
-                   let uu____2759 = l1.FStar_Syntax_Syntax.lcomp_as_comp ()
+                (fun uu____2789  ->
+                   let uu____2790 = l1.FStar_Syntax_Syntax.lcomp_as_comp ()
                       in
-                   FStar_Syntax_Subst.subst_comp s uu____2759)
+                   FStar_Syntax_Subst.subst_comp s uu____2790)
             }  in
           Some (FStar_Util.Inl l2)
-      | uu____2768 -> l  in
+      | uu____2799 -> l  in
     let rec aux t1 abs_body_lcomp =
-      let uu____2806 =
-        let uu____2807 =
-          let uu____2810 = FStar_Syntax_Subst.compress t1  in
-          FStar_All.pipe_left unascribe uu____2810  in
-        uu____2807.FStar_Syntax_Syntax.n  in
-      match uu____2806 with
+      let uu____2837 =
+        let uu____2838 =
+          let uu____2841 = FStar_Syntax_Subst.compress t1  in
+          FStar_All.pipe_left unascribe uu____2841  in
+        uu____2838.FStar_Syntax_Syntax.n  in
+      match uu____2837 with
       | FStar_Syntax_Syntax.Tm_abs (bs,t2,what) ->
-          let uu____2848 = aux t2 what  in
-          (match uu____2848 with
+          let uu____2879 = aux t2 what  in
+          (match uu____2879 with
            | (bs',t3,what1) -> ((FStar_List.append bs bs'), t3, what1))
-      | uu____2905 -> ([], t1, abs_body_lcomp)  in
-    let uu____2917 = aux t None  in
-    match uu____2917 with
+      | uu____2936 -> ([], t1, abs_body_lcomp)  in
+    let uu____2948 = aux t None  in
+    match uu____2948 with
     | (bs,t1,abs_body_lcomp) ->
-        let uu____2965 = FStar_Syntax_Subst.open_term' bs t1  in
-        (match uu____2965 with
+        let uu____2996 = FStar_Syntax_Subst.open_term' bs t1  in
+        (match uu____2996 with
          | (bs1,t2,opening) ->
              let abs_body_lcomp1 = subst_lcomp_opt opening abs_body_lcomp  in
              (bs1, t2, abs_body_lcomp1))
@@ -1327,7 +1342,7 @@ let close_univs_and_mk_letbinding :
               let def1 =
                 match (recs, univ_vars) with
                 | (None ,_)|(_,[]) -> def
-                | (Some fvs,uu____3065) ->
+                | (Some fvs,uu____3096) ->
                     let universes =
                       FStar_All.pipe_right univ_vars
                         (FStar_List.map
@@ -1359,20 +1374,20 @@ let open_univ_vars_binders_and_comp :
       fun c  ->
         match binders with
         | [] ->
-            let uu____3126 = FStar_Syntax_Subst.open_univ_vars_comp uvs c  in
-            (match uu____3126 with | (uvs1,c1) -> (uvs1, [], c1))
-        | uu____3142 ->
+            let uu____3157 = FStar_Syntax_Subst.open_univ_vars_comp uvs c  in
+            (match uu____3157 with | (uvs1,c1) -> (uvs1, [], c1))
+        | uu____3173 ->
             let t' = arrow binders c  in
-            let uu____3147 = FStar_Syntax_Subst.open_univ_vars uvs t'  in
-            (match uu____3147 with
+            let uu____3178 = FStar_Syntax_Subst.open_univ_vars uvs t'  in
+            (match uu____3178 with
              | (uvs1,t'1) ->
-                 let uu____3158 =
-                   let uu____3159 = FStar_Syntax_Subst.compress t'1  in
-                   uu____3159.FStar_Syntax_Syntax.n  in
-                 (match uu____3158 with
+                 let uu____3189 =
+                   let uu____3190 = FStar_Syntax_Subst.compress t'1  in
+                   uu____3190.FStar_Syntax_Syntax.n  in
+                 (match uu____3189 with
                   | FStar_Syntax_Syntax.Tm_arrow (binders1,c1) ->
                       (uvs1, binders1, c1)
-                  | uu____3185 -> failwith "Impossible"))
+                  | uu____3216 -> failwith "Impossible"))
   
 let is_tuple_constructor : FStar_Syntax_Syntax.typ -> Prims.bool =
   fun t  ->
@@ -1381,32 +1396,32 @@ let is_tuple_constructor : FStar_Syntax_Syntax.typ -> Prims.bool =
         FStar_Util.starts_with
           ((fv.FStar_Syntax_Syntax.fv_name).FStar_Syntax_Syntax.v).FStar_Ident.str
           "Prims.tuple"
-    | uu____3200 -> false
+    | uu____3231 -> false
   
 let mk_tuple_lid : Prims.int -> FStar_Range.range -> FStar_Ident.lident =
   fun n1  ->
     fun r  ->
       let t =
-        let uu____3208 = FStar_Util.string_of_int n1  in
-        FStar_Util.format1 "tuple%s" uu____3208  in
-      let uu____3209 = FStar_Syntax_Const.pconst t  in
-      FStar_Ident.set_lid_range uu____3209 r
+        let uu____3239 = FStar_Util.string_of_int n1  in
+        FStar_Util.format1 "tuple%s" uu____3239  in
+      let uu____3240 = FStar_Syntax_Const.pconst t  in
+      FStar_Ident.set_lid_range uu____3240 r
   
 let mk_tuple_data_lid : Prims.int -> FStar_Range.range -> FStar_Ident.lident
   =
   fun n1  ->
     fun r  ->
       let t =
-        let uu____3217 = FStar_Util.string_of_int n1  in
-        FStar_Util.format1 "Mktuple%s" uu____3217  in
-      let uu____3218 = FStar_Syntax_Const.pconst t  in
-      FStar_Ident.set_lid_range uu____3218 r
+        let uu____3248 = FStar_Util.string_of_int n1  in
+        FStar_Util.format1 "Mktuple%s" uu____3248  in
+      let uu____3249 = FStar_Syntax_Const.pconst t  in
+      FStar_Ident.set_lid_range uu____3249 r
   
 let is_tuple_data_lid : FStar_Ident.lident -> Prims.int -> Prims.bool =
   fun f  ->
     fun n1  ->
-      let uu____3225 = mk_tuple_data_lid n1 FStar_Range.dummyRange  in
-      FStar_Ident.lid_equals f uu____3225
+      let uu____3256 = mk_tuple_data_lid n1 FStar_Range.dummyRange  in
+      FStar_Ident.lid_equals f uu____3256
   
 let is_tuple_data_lid' : FStar_Ident.lident -> Prims.bool =
   fun f  ->
@@ -1430,26 +1445,26 @@ let is_dtuple_constructor : FStar_Syntax_Syntax.typ -> Prims.bool =
     | FStar_Syntax_Syntax.Tm_fvar fv ->
         is_dtuple_constructor_lid
           (fv.FStar_Syntax_Syntax.fv_name).FStar_Syntax_Syntax.v
-    | uu____3243 -> false
+    | uu____3274 -> false
   
 let mk_dtuple_lid : Prims.int -> FStar_Range.range -> FStar_Ident.lident =
   fun n1  ->
     fun r  ->
       let t =
-        let uu____3251 = FStar_Util.string_of_int n1  in
-        FStar_Util.format1 "dtuple%s" uu____3251  in
-      let uu____3252 = FStar_Syntax_Const.pconst t  in
-      FStar_Ident.set_lid_range uu____3252 r
+        let uu____3282 = FStar_Util.string_of_int n1  in
+        FStar_Util.format1 "dtuple%s" uu____3282  in
+      let uu____3283 = FStar_Syntax_Const.pconst t  in
+      FStar_Ident.set_lid_range uu____3283 r
   
 let mk_dtuple_data_lid : Prims.int -> FStar_Range.range -> FStar_Ident.lident
   =
   fun n1  ->
     fun r  ->
       let t =
-        let uu____3260 = FStar_Util.string_of_int n1  in
-        FStar_Util.format1 "Mkdtuple%s" uu____3260  in
-      let uu____3261 = FStar_Syntax_Const.pconst t  in
-      FStar_Ident.set_lid_range uu____3261 r
+        let uu____3291 = FStar_Util.string_of_int n1  in
+        FStar_Util.format1 "Mkdtuple%s" uu____3291  in
+      let uu____3292 = FStar_Syntax_Const.pconst t  in
+      FStar_Ident.set_lid_range uu____3292 r
   
 let is_dtuple_data_lid' : FStar_Ident.lident -> Prims.bool =
   fun f  -> FStar_Util.starts_with (FStar_Ident.text_of_lid f) "Mkdtuple" 
@@ -1474,25 +1489,25 @@ let is_constructor :
   FStar_Syntax_Syntax.term -> FStar_Ident.lident -> Prims.bool =
   fun t  ->
     fun lid  ->
-      let uu____3299 =
-        let uu____3300 = pre_typ t  in uu____3300.FStar_Syntax_Syntax.n  in
-      match uu____3299 with
+      let uu____3330 =
+        let uu____3331 = pre_typ t  in uu____3331.FStar_Syntax_Syntax.n  in
+      match uu____3330 with
       | FStar_Syntax_Syntax.Tm_fvar tc ->
           FStar_Ident.lid_equals
             (tc.FStar_Syntax_Syntax.fv_name).FStar_Syntax_Syntax.v lid
-      | uu____3308 -> false
+      | uu____3339 -> false
   
 let rec is_constructed_typ :
   FStar_Syntax_Syntax.term -> FStar_Ident.lident -> Prims.bool =
   fun t  ->
     fun lid  ->
-      let uu____3315 =
-        let uu____3316 = pre_typ t  in uu____3316.FStar_Syntax_Syntax.n  in
-      match uu____3315 with
-      | FStar_Syntax_Syntax.Tm_fvar uu____3319 -> is_constructor t lid
-      | FStar_Syntax_Syntax.Tm_app (t1,uu____3321) ->
+      let uu____3346 =
+        let uu____3347 = pre_typ t  in uu____3347.FStar_Syntax_Syntax.n  in
+      match uu____3346 with
+      | FStar_Syntax_Syntax.Tm_fvar uu____3350 -> is_constructor t lid
+      | FStar_Syntax_Syntax.Tm_app (t1,uu____3352) ->
           is_constructed_typ t1 lid
-      | uu____3336 -> false
+      | uu____3367 -> false
   
 let rec get_tycon :
   FStar_Syntax_Syntax.term -> FStar_Syntax_Syntax.term Prims.option =
@@ -1502,8 +1517,8 @@ let rec get_tycon :
     | FStar_Syntax_Syntax.Tm_bvar _
       |FStar_Syntax_Syntax.Tm_name _|FStar_Syntax_Syntax.Tm_fvar _ -> 
         Some t1
-    | FStar_Syntax_Syntax.Tm_app (t2,uu____3347) -> get_tycon t2
-    | uu____3362 -> None
+    | FStar_Syntax_Syntax.Tm_app (t2,uu____3378) -> get_tycon t2
+    | uu____3393 -> None
   
 let is_interpreted : FStar_Ident.lident -> Prims.bool =
   fun l  ->
@@ -1546,17 +1561,17 @@ let type_u :
     ((FStar_Syntax_Syntax.term',FStar_Syntax_Syntax.term')
       FStar_Syntax_Syntax.syntax * FStar_Syntax_Syntax.universe)
   =
-  fun uu____3392  ->
+  fun uu____3423  ->
     let u =
-      let uu____3396 = FStar_Unionfind.fresh None  in
+      let uu____3427 = FStar_Unionfind.fresh None  in
       FStar_All.pipe_left (fun _0_26  -> FStar_Syntax_Syntax.U_unif _0_26)
-        uu____3396
+        uu____3427
        in
-    let uu____3402 =
+    let uu____3433 =
       (FStar_Syntax_Syntax.mk (FStar_Syntax_Syntax.Tm_type u)) None
         FStar_Range.dummyRange
        in
-    (uu____3402, u)
+    (uu____3433, u)
   
 let type_at_u :
   FStar_Syntax_Syntax.universe ->
@@ -1598,55 +1613,55 @@ let mk_conj_opt :
       match phi1 with
       | None  -> Some phi2
       | Some phi11 ->
-          let uu____3440 =
-            let uu____3443 =
+          let uu____3471 =
+            let uu____3474 =
               FStar_Range.union_ranges phi11.FStar_Syntax_Syntax.pos
                 phi2.FStar_Syntax_Syntax.pos
                in
-            let uu____3444 =
-              let uu____3447 =
-                let uu____3448 =
-                  let uu____3458 =
-                    let uu____3460 = FStar_Syntax_Syntax.as_arg phi11  in
-                    let uu____3461 =
-                      let uu____3463 = FStar_Syntax_Syntax.as_arg phi2  in
-                      [uu____3463]  in
-                    uu____3460 :: uu____3461  in
-                  (tand, uu____3458)  in
-                FStar_Syntax_Syntax.Tm_app uu____3448  in
-              FStar_Syntax_Syntax.mk uu____3447  in
-            uu____3444 None uu____3443  in
-          Some uu____3440
+            let uu____3475 =
+              let uu____3478 =
+                let uu____3479 =
+                  let uu____3489 =
+                    let uu____3491 = FStar_Syntax_Syntax.as_arg phi11  in
+                    let uu____3492 =
+                      let uu____3494 = FStar_Syntax_Syntax.as_arg phi2  in
+                      [uu____3494]  in
+                    uu____3491 :: uu____3492  in
+                  (tand, uu____3489)  in
+                FStar_Syntax_Syntax.Tm_app uu____3479  in
+              FStar_Syntax_Syntax.mk uu____3478  in
+            uu____3475 None uu____3474  in
+          Some uu____3471
   
 let mk_binop op_t phi1 phi2 =
-  let uu____3498 =
+  let uu____3529 =
     FStar_Range.union_ranges phi1.FStar_Syntax_Syntax.pos
       phi2.FStar_Syntax_Syntax.pos
      in
-  let uu____3499 =
-    let uu____3502 =
-      let uu____3503 =
-        let uu____3513 =
-          let uu____3515 = FStar_Syntax_Syntax.as_arg phi1  in
-          let uu____3516 =
-            let uu____3518 = FStar_Syntax_Syntax.as_arg phi2  in [uu____3518]
+  let uu____3530 =
+    let uu____3533 =
+      let uu____3534 =
+        let uu____3544 =
+          let uu____3546 = FStar_Syntax_Syntax.as_arg phi1  in
+          let uu____3547 =
+            let uu____3549 = FStar_Syntax_Syntax.as_arg phi2  in [uu____3549]
              in
-          uu____3515 :: uu____3516  in
-        (op_t, uu____3513)  in
-      FStar_Syntax_Syntax.Tm_app uu____3503  in
-    FStar_Syntax_Syntax.mk uu____3502  in
-  uu____3499 None uu____3498 
+          uu____3546 :: uu____3547  in
+        (op_t, uu____3544)  in
+      FStar_Syntax_Syntax.Tm_app uu____3534  in
+    FStar_Syntax_Syntax.mk uu____3533  in
+  uu____3530 None uu____3529 
 let mk_neg phi =
-  let uu____3539 =
-    let uu____3542 =
-      let uu____3543 =
-        let uu____3553 =
-          let uu____3555 = FStar_Syntax_Syntax.as_arg phi  in [uu____3555]
+  let uu____3570 =
+    let uu____3573 =
+      let uu____3574 =
+        let uu____3584 =
+          let uu____3586 = FStar_Syntax_Syntax.as_arg phi  in [uu____3586]
            in
-        (t_not, uu____3553)  in
-      FStar_Syntax_Syntax.Tm_app uu____3543  in
-    FStar_Syntax_Syntax.mk uu____3542  in
-  uu____3539 None phi.FStar_Syntax_Syntax.pos 
+        (t_not, uu____3584)  in
+      FStar_Syntax_Syntax.Tm_app uu____3574  in
+    FStar_Syntax_Syntax.mk uu____3573  in
+  uu____3570 None phi.FStar_Syntax_Syntax.pos 
 let mk_conj phi1 phi2 = mk_binop tand phi1 phi2 
 let mk_conj_l :
   FStar_Syntax_Syntax.term Prims.list -> FStar_Syntax_Syntax.term =
@@ -1671,59 +1686,59 @@ let mk_imp :
   =
   fun phi1  ->
     fun phi2  ->
-      let uu____3615 =
-        let uu____3616 = FStar_Syntax_Subst.compress phi1  in
-        uu____3616.FStar_Syntax_Syntax.n  in
-      match uu____3615 with
+      let uu____3646 =
+        let uu____3647 = FStar_Syntax_Subst.compress phi1  in
+        uu____3647.FStar_Syntax_Syntax.n  in
+      match uu____3646 with
       | FStar_Syntax_Syntax.Tm_fvar tc when
           FStar_Syntax_Syntax.fv_eq_lid tc FStar_Syntax_Const.false_lid ->
           t_true
       | FStar_Syntax_Syntax.Tm_fvar tc when
           FStar_Syntax_Syntax.fv_eq_lid tc FStar_Syntax_Const.true_lid ->
           phi2
-      | uu____3621 ->
-          let uu____3622 =
-            let uu____3623 = FStar_Syntax_Subst.compress phi2  in
-            uu____3623.FStar_Syntax_Syntax.n  in
-          (match uu____3622 with
+      | uu____3652 ->
+          let uu____3653 =
+            let uu____3654 = FStar_Syntax_Subst.compress phi2  in
+            uu____3654.FStar_Syntax_Syntax.n  in
+          (match uu____3653 with
            | FStar_Syntax_Syntax.Tm_fvar tc when
                (FStar_Syntax_Syntax.fv_eq_lid tc FStar_Syntax_Const.true_lid)
                  ||
                  (FStar_Syntax_Syntax.fv_eq_lid tc
                     FStar_Syntax_Const.false_lid)
                -> phi2
-           | uu____3627 -> mk_binop timp phi1 phi2)
+           | uu____3658 -> mk_binop timp phi1 phi2)
   
 let mk_iff phi1 phi2 = mk_binop tiff phi1 phi2 
 let b2t e =
-  let uu____3651 =
-    let uu____3654 =
-      let uu____3655 =
-        let uu____3665 =
-          let uu____3667 = FStar_Syntax_Syntax.as_arg e  in [uu____3667]  in
-        (b2t_v, uu____3665)  in
-      FStar_Syntax_Syntax.Tm_app uu____3655  in
-    FStar_Syntax_Syntax.mk uu____3654  in
-  uu____3651 None e.FStar_Syntax_Syntax.pos 
+  let uu____3682 =
+    let uu____3685 =
+      let uu____3686 =
+        let uu____3696 =
+          let uu____3698 = FStar_Syntax_Syntax.as_arg e  in [uu____3698]  in
+        (b2t_v, uu____3696)  in
+      FStar_Syntax_Syntax.Tm_app uu____3686  in
+    FStar_Syntax_Syntax.mk uu____3685  in
+  uu____3682 None e.FStar_Syntax_Syntax.pos 
 let teq : FStar_Syntax_Syntax.term = fvar_const FStar_Syntax_Const.eq2_lid 
 let mk_untyped_eq2 e1 e2 =
-  let uu____3691 =
+  let uu____3722 =
     FStar_Range.union_ranges e1.FStar_Syntax_Syntax.pos
       e2.FStar_Syntax_Syntax.pos
      in
-  let uu____3692 =
-    let uu____3695 =
-      let uu____3696 =
-        let uu____3706 =
-          let uu____3708 = FStar_Syntax_Syntax.as_arg e1  in
-          let uu____3709 =
-            let uu____3711 = FStar_Syntax_Syntax.as_arg e2  in [uu____3711]
+  let uu____3723 =
+    let uu____3726 =
+      let uu____3727 =
+        let uu____3737 =
+          let uu____3739 = FStar_Syntax_Syntax.as_arg e1  in
+          let uu____3740 =
+            let uu____3742 = FStar_Syntax_Syntax.as_arg e2  in [uu____3742]
              in
-          uu____3708 :: uu____3709  in
-        (teq, uu____3706)  in
-      FStar_Syntax_Syntax.Tm_app uu____3696  in
-    FStar_Syntax_Syntax.mk uu____3695  in
-  uu____3692 None uu____3691 
+          uu____3739 :: uu____3740  in
+        (teq, uu____3737)  in
+      FStar_Syntax_Syntax.Tm_app uu____3727  in
+    FStar_Syntax_Syntax.mk uu____3726  in
+  uu____3723 None uu____3722 
 let mk_eq2 :
   FStar_Syntax_Syntax.universe ->
     FStar_Syntax_Syntax.typ ->
@@ -1737,26 +1752,26 @@ let mk_eq2 :
       fun e1  ->
         fun e2  ->
           let eq_inst = FStar_Syntax_Syntax.mk_Tm_uinst teq [u]  in
-          let uu____3734 =
+          let uu____3765 =
             FStar_Range.union_ranges e1.FStar_Syntax_Syntax.pos
               e2.FStar_Syntax_Syntax.pos
              in
-          let uu____3735 =
-            let uu____3738 =
-              let uu____3739 =
-                let uu____3749 =
-                  let uu____3751 = FStar_Syntax_Syntax.iarg t  in
-                  let uu____3752 =
-                    let uu____3754 = FStar_Syntax_Syntax.as_arg e1  in
-                    let uu____3755 =
-                      let uu____3757 = FStar_Syntax_Syntax.as_arg e2  in
-                      [uu____3757]  in
-                    uu____3754 :: uu____3755  in
-                  uu____3751 :: uu____3752  in
-                (eq_inst, uu____3749)  in
-              FStar_Syntax_Syntax.Tm_app uu____3739  in
-            FStar_Syntax_Syntax.mk uu____3738  in
-          uu____3735 None uu____3734
+          let uu____3766 =
+            let uu____3769 =
+              let uu____3770 =
+                let uu____3780 =
+                  let uu____3782 = FStar_Syntax_Syntax.iarg t  in
+                  let uu____3783 =
+                    let uu____3785 = FStar_Syntax_Syntax.as_arg e1  in
+                    let uu____3786 =
+                      let uu____3788 = FStar_Syntax_Syntax.as_arg e2  in
+                      [uu____3788]  in
+                    uu____3785 :: uu____3786  in
+                  uu____3782 :: uu____3783  in
+                (eq_inst, uu____3780)  in
+              FStar_Syntax_Syntax.Tm_app uu____3770  in
+            FStar_Syntax_Syntax.mk uu____3769  in
+          uu____3766 None uu____3765
   
 let mk_has_type t x t' =
   let t_has_type = fvar_const FStar_Syntax_Const.has_type_lid  in
@@ -1767,22 +1782,22 @@ let mk_has_type t x t' =
            [FStar_Syntax_Syntax.U_zero; FStar_Syntax_Syntax.U_zero])) None
       FStar_Range.dummyRange
      in
-  let uu____3795 =
-    let uu____3798 =
-      let uu____3799 =
-        let uu____3809 =
-          let uu____3811 = FStar_Syntax_Syntax.iarg t  in
-          let uu____3812 =
-            let uu____3814 = FStar_Syntax_Syntax.as_arg x  in
-            let uu____3815 =
-              let uu____3817 = FStar_Syntax_Syntax.as_arg t'  in [uu____3817]
+  let uu____3826 =
+    let uu____3829 =
+      let uu____3830 =
+        let uu____3840 =
+          let uu____3842 = FStar_Syntax_Syntax.iarg t  in
+          let uu____3843 =
+            let uu____3845 = FStar_Syntax_Syntax.as_arg x  in
+            let uu____3846 =
+              let uu____3848 = FStar_Syntax_Syntax.as_arg t'  in [uu____3848]
                in
-            uu____3814 :: uu____3815  in
-          uu____3811 :: uu____3812  in
-        (t_has_type1, uu____3809)  in
-      FStar_Syntax_Syntax.Tm_app uu____3799  in
-    FStar_Syntax_Syntax.mk uu____3798  in
-  uu____3795 None FStar_Range.dummyRange 
+            uu____3845 :: uu____3846  in
+          uu____3842 :: uu____3843  in
+        (t_has_type1, uu____3840)  in
+      FStar_Syntax_Syntax.Tm_app uu____3830  in
+    FStar_Syntax_Syntax.mk uu____3829  in
+  uu____3826 None FStar_Range.dummyRange 
 let lex_t : FStar_Syntax_Syntax.term =
   fvar_const FStar_Syntax_Const.lex_t_lid 
 let lex_top : FStar_Syntax_Syntax.term =
@@ -1810,7 +1825,7 @@ let lc_tot_type0 : FStar_Syntax_Syntax.lcomp =
     FStar_Syntax_Syntax.lcomp_res_typ = ktype0;
     FStar_Syntax_Syntax.lcomp_cflags = [FStar_Syntax_Syntax.TOTAL];
     FStar_Syntax_Syntax.lcomp_as_comp =
-      (fun uu____3833  -> FStar_Syntax_Syntax.mk_Total ktype0)
+      (fun uu____3864  -> FStar_Syntax_Syntax.mk_Total ktype0)
   } 
 let mk_forall :
   FStar_Syntax_Syntax.bv ->
@@ -1820,27 +1835,27 @@ let mk_forall :
   =
   fun x  ->
     fun body  ->
-      let uu____3840 =
-        let uu____3843 =
-          let uu____3844 =
-            let uu____3854 =
-              let uu____3856 =
+      let uu____3871 =
+        let uu____3874 =
+          let uu____3875 =
+            let uu____3885 =
+              let uu____3887 =
                 FStar_Syntax_Syntax.iarg x.FStar_Syntax_Syntax.sort  in
-              let uu____3857 =
-                let uu____3859 =
-                  let uu____3860 =
-                    let uu____3861 =
-                      let uu____3865 = FStar_Syntax_Syntax.mk_binder x  in
-                      [uu____3865]  in
-                    abs uu____3861 body (Some (FStar_Util.Inl lc_tot_type0))
+              let uu____3888 =
+                let uu____3890 =
+                  let uu____3891 =
+                    let uu____3892 =
+                      let uu____3896 = FStar_Syntax_Syntax.mk_binder x  in
+                      [uu____3896]  in
+                    abs uu____3892 body (Some (FStar_Util.Inl lc_tot_type0))
                      in
-                  FStar_Syntax_Syntax.as_arg uu____3860  in
-                [uu____3859]  in
-              uu____3856 :: uu____3857  in
-            (tforall, uu____3854)  in
-          FStar_Syntax_Syntax.Tm_app uu____3844  in
-        FStar_Syntax_Syntax.mk uu____3843  in
-      uu____3840 None FStar_Range.dummyRange
+                  FStar_Syntax_Syntax.as_arg uu____3891  in
+                [uu____3890]  in
+              uu____3887 :: uu____3888  in
+            (tforall, uu____3885)  in
+          FStar_Syntax_Syntax.Tm_app uu____3875  in
+        FStar_Syntax_Syntax.mk uu____3874  in
+      uu____3871 None FStar_Range.dummyRange
   
 let rec close_forall :
   FStar_Syntax_Syntax.binder Prims.list ->
@@ -1851,39 +1866,39 @@ let rec close_forall :
       FStar_List.fold_right
         (fun b  ->
            fun f1  ->
-             let uu____3893 = FStar_Syntax_Syntax.is_null_binder b  in
-             if uu____3893 then f1 else mk_forall (Prims.fst b) f1) bs f
+             let uu____3924 = FStar_Syntax_Syntax.is_null_binder b  in
+             if uu____3924 then f1 else mk_forall (Prims.fst b) f1) bs f
   
 let rec is_wild_pat p =
   match p.FStar_Syntax_Syntax.v with
-  | FStar_Syntax_Syntax.Pat_wild uu____3906 -> true
-  | uu____3907 -> false 
+  | FStar_Syntax_Syntax.Pat_wild uu____3937 -> true
+  | uu____3938 -> false 
 let if_then_else b t1 t2 =
   let then_branch =
-    let uu____3950 =
+    let uu____3981 =
       FStar_Syntax_Syntax.withinfo
         (FStar_Syntax_Syntax.Pat_constant (FStar_Const.Const_bool true))
         FStar_Syntax_Syntax.tun.FStar_Syntax_Syntax.n
         t1.FStar_Syntax_Syntax.pos
        in
-    (uu____3950, None, t1)  in
+    (uu____3981, None, t1)  in
   let else_branch =
-    let uu____3973 =
+    let uu____4004 =
       FStar_Syntax_Syntax.withinfo
         (FStar_Syntax_Syntax.Pat_constant (FStar_Const.Const_bool false))
         FStar_Syntax_Syntax.tun.FStar_Syntax_Syntax.n
         t2.FStar_Syntax_Syntax.pos
        in
-    (uu____3973, None, t2)  in
-  let uu____3985 =
-    let uu____3986 =
+    (uu____4004, None, t2)  in
+  let uu____4016 =
+    let uu____4017 =
       FStar_Range.union_ranges t1.FStar_Syntax_Syntax.pos
         t2.FStar_Syntax_Syntax.pos
        in
-    FStar_Range.union_ranges b.FStar_Syntax_Syntax.pos uu____3986  in
+    FStar_Range.union_ranges b.FStar_Syntax_Syntax.pos uu____4017  in
   FStar_Syntax_Syntax.mk
     (FStar_Syntax_Syntax.Tm_match (b, [then_branch; else_branch])) None
-    uu____3985
+    uu____4016
   
 type qpats = FStar_Syntax_Syntax.args Prims.list
 type connective =
@@ -1892,7 +1907,7 @@ type connective =
   | BaseConn of (FStar_Ident.lident * FStar_Syntax_Syntax.args) 
 let uu___is_QAll : connective -> Prims.bool =
   fun projectee  ->
-    match projectee with | QAll _0 -> true | uu____4059 -> false
+    match projectee with | QAll _0 -> true | uu____4090 -> false
   
 let __proj__QAll__item___0 :
   connective ->
@@ -1900,7 +1915,7 @@ let __proj__QAll__item___0 :
   = fun projectee  -> match projectee with | QAll _0 -> _0 
 let uu___is_QEx : connective -> Prims.bool =
   fun projectee  ->
-    match projectee with | QEx _0 -> true | uu____4083 -> false
+    match projectee with | QEx _0 -> true | uu____4114 -> false
   
 let __proj__QEx__item___0 :
   connective ->
@@ -1908,7 +1923,7 @@ let __proj__QEx__item___0 :
   = fun projectee  -> match projectee with | QEx _0 -> _0 
 let uu___is_BaseConn : connective -> Prims.bool =
   fun projectee  ->
-    match projectee with | BaseConn _0 -> true | uu____4106 -> false
+    match projectee with | BaseConn _0 -> true | uu____4137 -> false
   
 let __proj__BaseConn__item___0 :
   connective -> (FStar_Ident.lident * FStar_Syntax_Syntax.args) =
@@ -1922,7 +1937,7 @@ let destruct_typ_as_formula :
       | FStar_Syntax_Syntax.Tm_meta (t,FStar_Syntax_Syntax.Meta_monadic _)
         |FStar_Syntax_Syntax.Tm_meta
         (t,FStar_Syntax_Syntax.Meta_monadic_lift _) -> unmeta_monadic t
-      | uu____4141 -> f2  in
+      | uu____4172 -> f2  in
     let destruct_base_conn f1 =
       let connectives =
         [(FStar_Syntax_Const.true_lid, (Prims.parse_int "0"));
@@ -1937,20 +1952,20 @@ let destruct_typ_as_formula :
         (FStar_Syntax_Const.eq2_lid, (Prims.parse_int "2"));
         (FStar_Syntax_Const.eq3_lid, (Prims.parse_int "4"));
         (FStar_Syntax_Const.eq3_lid, (Prims.parse_int "2"))]  in
-      let rec aux f2 uu____4186 =
-        match uu____4186 with
+      let rec aux f2 uu____4217 =
+        match uu____4217 with
         | (lid,arity) ->
-            let uu____4192 =
-              let uu____4202 = unmeta_monadic f2  in head_and_args uu____4202
+            let uu____4223 =
+              let uu____4233 = unmeta_monadic f2  in head_and_args uu____4233
                in
-            (match uu____4192 with
+            (match uu____4223 with
              | (t,args) ->
                  let t1 = un_uinst t  in
-                 let uu____4221 =
+                 let uu____4252 =
                    (is_constructor t1 lid) &&
                      ((FStar_List.length args) = arity)
                     in
-                 if uu____4221 then Some (BaseConn (lid, args)) else None)
+                 if uu____4252 then Some (BaseConn (lid, args)) else None)
          in
       FStar_Util.find_map connectives (aux f1)  in
     let patterns t =
@@ -1958,11 +1973,11 @@ let destruct_typ_as_formula :
       match t1.FStar_Syntax_Syntax.n with
       | FStar_Syntax_Syntax.Tm_meta
           (t2,FStar_Syntax_Syntax.Meta_pattern pats) ->
-          let uu____4272 = FStar_Syntax_Subst.compress t2  in
-          (pats, uu____4272)
-      | uu____4279 ->
-          let uu____4280 = FStar_Syntax_Subst.compress t1  in
-          ([], uu____4280)
+          let uu____4303 = FStar_Syntax_Subst.compress t2  in
+          (pats, uu____4303)
+      | uu____4310 ->
+          let uu____4311 = FStar_Syntax_Subst.compress t1  in
+          ([], uu____4311)
        in
     let destruct_q_conn t =
       let is_q fa fv =
@@ -1971,23 +1986,23 @@ let destruct_typ_as_formula :
         else is_exists (fv.FStar_Syntax_Syntax.fv_name).FStar_Syntax_Syntax.v
          in
       let flat t1 =
-        let uu____4322 = head_and_args t1  in
-        match uu____4322 with
+        let uu____4353 = head_and_args t1  in
+        match uu____4353 with
         | (t2,args) ->
-            let uu____4353 = un_uinst t2  in
-            let uu____4354 =
+            let uu____4384 = un_uinst t2  in
+            let uu____4385 =
               FStar_All.pipe_right args
                 (FStar_List.map
-                   (fun uu____4370  ->
-                      match uu____4370 with
+                   (fun uu____4401  ->
+                      match uu____4401 with
                       | (t3,imp) ->
-                          let uu____4377 = unascribe t3  in (uu____4377, imp)))
+                          let uu____4408 = unascribe t3  in (uu____4408, imp)))
                in
-            (uu____4353, uu____4354)
+            (uu____4384, uu____4385)
          in
       let rec aux qopt out t1 =
-        let uu____4400 = let uu____4409 = flat t1  in (qopt, uu____4409)  in
-        match uu____4400 with
+        let uu____4431 = let uu____4440 = flat t1  in (qopt, uu____4440)  in
+        match uu____4431 with
         | (Some
            fa,({ FStar_Syntax_Syntax.n = FStar_Syntax_Syntax.Tm_fvar tc;
                  FStar_Syntax_Syntax.tk = _; FStar_Syntax_Syntax.pos = _;
@@ -2047,22 +2062,22 @@ let destruct_typ_as_formula :
                  (is_forall
                     (tc.FStar_Syntax_Syntax.fv_name).FStar_Syntax_Syntax.v))
               (b :: out) t2
-        | (Some b,uu____4668) ->
+        | (Some b,uu____4699) ->
             let bs = FStar_List.rev out  in
-            let uu____4686 = FStar_Syntax_Subst.open_term bs t1  in
-            (match uu____4686 with
+            let uu____4717 = FStar_Syntax_Subst.open_term bs t1  in
+            (match uu____4717 with
              | (bs1,t2) ->
-                 let uu____4692 = patterns t2  in
-                 (match uu____4692 with
+                 let uu____4723 = patterns t2  in
+                 (match uu____4723 with
                   | (pats,body) ->
                       if b
                       then Some (QAll (bs1, pats, body))
                       else Some (QEx (bs1, pats, body))))
-        | uu____4730 -> None  in
+        | uu____4761 -> None  in
       aux None [] t  in
     let phi = unmeta_monadic f  in
-    let uu____4742 = destruct_base_conn phi  in
-    match uu____4742 with | Some b -> Some b | None  -> destruct_q_conn phi
+    let uu____4773 = destruct_base_conn phi  in
+    match uu____4773 with | Some b -> Some b | None  -> destruct_q_conn phi
   
 let action_as_lb :
   FStar_Ident.lident ->
@@ -2071,13 +2086,13 @@ let action_as_lb :
   fun eff_lid  ->
     fun a  ->
       let lb =
-        let uu____4753 =
-          let uu____4756 =
+        let uu____4784 =
+          let uu____4787 =
             FStar_Syntax_Syntax.lid_as_fv a.FStar_Syntax_Syntax.action_name
               FStar_Syntax_Syntax.Delta_equational None
              in
-          FStar_Util.Inr uu____4756  in
-        close_univs_and_mk_letbinding None uu____4753
+          FStar_Util.Inr uu____4787  in
+        close_univs_and_mk_letbinding None uu____4784
           a.FStar_Syntax_Syntax.action_univs a.FStar_Syntax_Syntax.action_typ
           FStar_Syntax_Const.effect_Tot_lid a.FStar_Syntax_Syntax.action_defn
          in
@@ -2094,21 +2109,21 @@ let mk_reify t =
       (FStar_Syntax_Syntax.Tm_constant FStar_Const.Const_reify) None
       t.FStar_Syntax_Syntax.pos
      in
-  let uu____4785 =
-    let uu____4788 =
-      let uu____4789 =
-        let uu____4799 =
-          let uu____4801 = FStar_Syntax_Syntax.as_arg t  in [uu____4801]  in
-        (reify_, uu____4799)  in
-      FStar_Syntax_Syntax.Tm_app uu____4789  in
-    FStar_Syntax_Syntax.mk uu____4788  in
-  uu____4785 None t.FStar_Syntax_Syntax.pos 
+  let uu____4816 =
+    let uu____4819 =
+      let uu____4820 =
+        let uu____4830 =
+          let uu____4832 = FStar_Syntax_Syntax.as_arg t  in [uu____4832]  in
+        (reify_, uu____4830)  in
+      FStar_Syntax_Syntax.Tm_app uu____4820  in
+    FStar_Syntax_Syntax.mk uu____4819  in
+  uu____4816 None t.FStar_Syntax_Syntax.pos 
 let rec delta_qualifier :
   FStar_Syntax_Syntax.term -> FStar_Syntax_Syntax.delta_depth =
   fun t  ->
     let t1 = FStar_Syntax_Subst.compress t  in
     match t1.FStar_Syntax_Syntax.n with
-    | FStar_Syntax_Syntax.Tm_delayed uu____4817 -> failwith "Impossible"
+    | FStar_Syntax_Syntax.Tm_delayed uu____4848 -> failwith "Impossible"
     | FStar_Syntax_Syntax.Tm_fvar fv -> fv.FStar_Syntax_Syntax.fv_delta
     | FStar_Syntax_Syntax.Tm_bvar _
       |FStar_Syntax_Syntax.Tm_name _
@@ -2146,39 +2161,39 @@ let incr_delta_qualifier :
   
 let is_unknown : FStar_Syntax_Syntax.term -> Prims.bool =
   fun t  ->
-    let uu____4923 =
-      let uu____4924 = FStar_Syntax_Subst.compress t  in
-      uu____4924.FStar_Syntax_Syntax.n  in
-    match uu____4923 with
+    let uu____4954 =
+      let uu____4955 = FStar_Syntax_Subst.compress t  in
+      uu____4955.FStar_Syntax_Syntax.n  in
+    match uu____4954 with
     | FStar_Syntax_Syntax.Tm_unknown  -> true
-    | uu____4927 -> false
+    | uu____4958 -> false
   
 let rec list_elements :
   FStar_Syntax_Syntax.term ->
     FStar_Syntax_Syntax.term Prims.list Prims.option
   =
   fun e  ->
-    let uu____4935 = let uu____4945 = unmeta e  in head_and_args uu____4945
+    let uu____4966 = let uu____4976 = unmeta e  in head_and_args uu____4976
        in
-    match uu____4935 with
+    match uu____4966 with
     | (head1,args) ->
-        let uu____4964 =
-          let uu____4972 =
-            let uu____4973 = un_uinst head1  in
-            uu____4973.FStar_Syntax_Syntax.n  in
-          (uu____4972, args)  in
-        (match uu____4964 with
-         | (FStar_Syntax_Syntax.Tm_fvar fv,uu____4984) when
+        let uu____4995 =
+          let uu____5003 =
+            let uu____5004 = un_uinst head1  in
+            uu____5004.FStar_Syntax_Syntax.n  in
+          (uu____5003, args)  in
+        (match uu____4995 with
+         | (FStar_Syntax_Syntax.Tm_fvar fv,uu____5015) when
              FStar_Syntax_Syntax.fv_eq_lid fv FStar_Syntax_Const.nil_lid ->
              Some []
          | (FStar_Syntax_Syntax.Tm_fvar
-            fv,uu____4997::(hd1,uu____4999)::(tl1,uu____5001)::[]) when
+            fv,uu____5028::(hd1,uu____5030)::(tl1,uu____5032)::[]) when
              FStar_Syntax_Syntax.fv_eq_lid fv FStar_Syntax_Const.cons_lid ->
-             let uu____5035 =
-               let uu____5039 =
-                 let uu____5043 = list_elements tl1  in
-                 FStar_Util.must uu____5043  in
-               hd1 :: uu____5039  in
-             Some uu____5035
-         | uu____5052 -> None)
+             let uu____5066 =
+               let uu____5070 =
+                 let uu____5074 = list_elements tl1  in
+                 FStar_Util.must uu____5074  in
+               hd1 :: uu____5070  in
+             Some uu____5066
+         | uu____5083 -> None)
   
